ulib/experimental/Steel.FramingReference.fsti
@@ -16,6 +16,7 @@
 
 module Steel.FramingReference
 open Steel.FramingEffect
+open Steel.FramingEffect.Atomic
 open Steel.Memory
 open Steel.FractionalPermission
 open FStar.Ghost
@@ -41,3 +42,27 @@ val write (#a:Type0) (#v:erased a) (r:ref a) (x:a)
 
 val free (#a:Type0) (#v:erased a) (r:ref a)
   : SteelT unit (pts_to r full_perm v) (fun _ -> emp)
+
+
+val share_atomic (#a:Type0) (#uses:_) (#p:perm) (#v:erased a) (r:ref a)
+  : SteelAtomic unit uses unobservable
+    (pts_to r p v)
+    (fun _ -> pts_to r (half_perm p) v `star` pts_to r (half_perm p) v)
+
+val gather_atomic (#a:Type0) (#uses:_) (#p0:perm) (#p1:perm) (#v0 #v1:erased a) (r:ref a)
+  : SteelAtomic (_:unit{v0 == v1}) uses unobservable
+    (pts_to r p0 v0 `star` pts_to r p1 v1)
+    (fun _ -> pts_to r (sum_perm p0 p1) v0)
+
+val cas (#t:eqtype)
+        (#uses:inames)
+        (r:ref t)
+        (v:Ghost.erased t)
+        (v_old:t)
+        (v_new:t)
+  : SteelAtomic
+        (b:bool{b <==> (Ghost.reveal v == v_old)})
+        uses
+        observable
+        (pts_to r full_perm v)
+        (fun b -> if b then pts_to r full_perm v_new else pts_to r full_perm v)
